Fixed dafny bug caused by boolean expressions. Fixed bug where outputstream blocked process execution. Fixed bug where incomplete grammar was being generated for some comparison operators. 'Equal' benchmark now works. Fixed a parser bug.

bin/Count.java
@@ -1,0 +1,57 @@
+import org.apache.spark.SparkConf;
+import org.apache.spark.api.java.JavaSparkContext;
+import org.apache.spark.api.java.JavaPairRDD;
+import org.apache.spark.api.java.JavaRDD;
+import org.apache.spark.api.java.function.Function2;
+import org.apache.spark.api.java.function.PairFlatMapFunction;
+import scala.Tuple2;
+import java.util.ArrayList;
+import java.util.Map;
+import java.util.List;
+import java.lang.Integer;
+
+public class Count {
+	
+	public static void main(String[] args) { countList(null); }
+	
+	public static int countList(List<Integer> data) {
+		int count = 0;
+		count = 0;
+		{
+			int i = 0;
+			i = 0;
+			boolean loop$0 = false;
+			loop$0 = false;
+			SparkConf conf = new SparkConf().setAppName("spark");
+			JavaSparkContext sc = new JavaSparkContext(conf);
+			
+			JavaRDD<java.lang.Integer> rdd_0_0 = sc.parallelize(data);
+			
+			final boolean loop0_final = loop$0;
+			
+			
+			JavaPairRDD<Integer, Integer> mapEmits = rdd_0_0.flatMapToPair(new PairFlatMapFunction<java.lang.Integer, Integer, Integer>() {
+				public Iterable<Tuple2<Integer, Integer>> call(java.lang.Integer data_i) throws Exception {
+					List<Tuple2<Integer, Integer>> emits = new ArrayList<Tuple2<Integer, Integer>>();
+					
+					emits.add(new Tuple2(0,1));
+					
+					
+					return emits;
+				}
+			});
+			
+			JavaPairRDD<Integer, Integer> reduceEmits = mapEmits.reduceByKey(new Function2<Integer,Integer,Integer>(){
+				public Integer call(Integer val1, Integer val2) throws Exception {
+					return val1 + val2;
+				}
+			});
+			
+			Map<Integer, Integer> output_rdd_0_0 = reduceEmits.collectAsMap();
+			count = output_rdd_0_0.get(0);
+		}
+		return count;
+	}
+	
+	public Count() { super(); }
+}
