bin/templates/dafny_skeleton.dfy
@@ -25,19 +25,19 @@ function mapper (<mapper-args-decl>) : <domap-emit-type>
 
 function doreduce(input: <domap-emit-type>, key: <doreduce-key-type>) : <output-type>
   ensures (|input| > 0 && input[0].0 == key) ==> 
-      doreduce(input, key) == <reduce-exp>
+      doreduce(input, key) == (<reduce-exp>)
   ensures (|input| > 0 && input[0].0 != key) ==> 
       doreduce(input, key) == doreduce(input[1..], key)
 {
   if input == [] then <reduce-init-value> 
-  else if input[0].0 == key then <reduce-exp>
+  else if input[0].0 == key then (<reduce-exp>)
   else doreduce(input[1..], key)
 }
 
 /******************************* HARNESS ************************************/  
 
 lemma Lemma2 (a: <domap-emit-type>, b: <domap-emit-type>, key: <doreduce-key-type>)
-  ensures doreduce(a+b,key) == <reduce-exp-lemma>
+  ensures doreduce(a+b,key) == (<reduce-exp-lemma>)
 {
   if a != []
   {
